template-coq/theories/Environment.v
@@ -13,6 +13,7 @@ Module Type Term.
   Parameter (tRel : nat -> term).
   Parameter (tSort : universe -> term).
   Parameter (tProd : name -> term -> term -> term).
+  Parameter (tLambda : name -> term -> term -> term).
   Parameter (tLetIn : name -> term -> term -> term -> term).
   Parameter (tInd : inductive -> universe_instance -> term).
 
@@ -103,6 +104,19 @@ Module Environment (T : Term).
   Notation " Γ  ,,, Γ' " :=
     (app_context Γ Γ') (at level 25, Γ' at next level, left associativity).
 
+  (** Make a lambda/let-in string of abstractions from a context [Γ], ending with term [t]. *)
+
+  Definition mkLambda_or_LetIn d t :=
+    match d.(decl_body) with
+    | None => tLambda d.(decl_name) d.(decl_type) t
+    | Some b => tLetIn d.(decl_name) b d.(decl_type) t
+    end.
+
+  Definition it_mkLambda_or_LetIn (l : context) (t : term) :=
+    List.fold_left (fun acc d => mkLambda_or_LetIn d acc) l t.
+
+  (** Make a prod/let-in string of abstractions from a context [Γ], ending with term [t]. *)
+
   Definition mkProd_or_LetIn d t :=
     match d.(decl_body) with
     | None => tProd d.(decl_name) d.(decl_type) t
@@ -111,6 +125,19 @@ Module Environment (T : Term).
 
   Definition it_mkProd_or_LetIn (l : context) (t : term) :=
     List.fold_left (fun acc d => mkProd_or_LetIn d acc) l t.
+
+  Definition map_decl f (d : context_decl) :=
+    {| decl_name := d.(decl_name);
+      decl_body := option_map f d.(decl_body);
+      decl_type := f d.(decl_type) |}.
+
+  Definition map_context f c :=
+    List.map (map_decl f) c.
+
+  Definition map_constant_body f decl :=
+    {| cst_type := f decl.(cst_type);
+       cst_body := option_map f decl.(cst_body);
+       cst_universes := decl.(cst_universes) |}.
 
   Fixpoint reln (l : list term) (p : nat) (Γ0 : list context_decl) {struct Γ0} : list term :=
     match Γ0 with
