pcuic/theories/PCUICUniverses.v
@@ -1,0 +1,87 @@
+(* Distributed under the terms of the MIT license.   *)
+
+From Coq Require Import Bool String List Program BinPos Compare_dec Arith Lia
+     Classes.CRelationClasses ProofIrrelevance.
+From MetaCoq.Template Require Import config Universes monad_utils utils BasicAst
+     AstUtils UnivSubst.
+From MetaCoq.PCUIC Require Import PCUICAst PCUICAstUtils PCUICInduction
+     PCUICReflect PCUICLiftSubst PCUICUtils.
+
+From Equations Require Import Equations.
+
+Require Import Equations.Prop.DepElim.
+Require Import Equations.Type.Relation_Properties.
+
+Local Set Keyed Unification.
+Set Equations With UIP.
+
+Require Import ssreflect ssrbool.
+
+Definition max_list (u : list universe) v : universe :=
+  List.fold_left (fun u v => Universe.sort_of_product v u) u v.
+
+Require Import Morphisms.
+Section UniverseLemmas.
+  Context {cf:checker_flags}.
+
+  Lemma NEL_forallb_app {A:Set} (P : A -> bool) l l' :
+    NEL.forallb P (NEL.app l l') =
+    NEL.forallb P l && NEL.forallb P l'.
+  Proof.
+    induction l.
+    - reflexivity.
+    - cbn. rewrite IHl. apply andb_assoc.
+  Qed.
+
+  Lemma is_prop_sup u s :
+    Universe.is_prop (Universe.sup u s)
+    = Universe.is_prop u && Universe.is_prop s.
+  Proof.
+    apply NEL_forallb_app.
+  Qed.
+
+  Ltac unfold_eq_universe
+    := unfold eq_universe in *; destruct check_univs; [intros v Hv|trivial].
+
+  Lemma sort_of_product_idem φ s
+    : eq_universe φ (Universe.sort_of_product s s) s.
+  Proof.
+    unfold Universe.sort_of_product. destruct (Universe.is_prop s).
+    - reflexivity.
+    - unfold_eq_universe. rewrite val_sup; lia.
+  Qed.
+
+  Lemma eq_universe_sup_assoc φ s1 s2 s3 :
+    eq_universe φ (Universe.sup s1 (Universe.sup s2 s3))
+                  (Universe.sup (Universe.sup s1 s2) s3).
+  Proof.
+    unfold_eq_universe. rewrite !val_sup; lia.
+  Qed.
+
+  Lemma eq_universe_sup_idem φ s :
+    eq_universe φ (Universe.sup s s) s.
+  Proof.
+    unfold_eq_universe. rewrite !val_sup; lia.
+  Qed.
+
+  Instance sup_eq_universe φ :
+    Proper (eq_universe φ ==> eq_universe φ ==> eq_universe φ) Universe.sup.
+  Proof.
+    intros s1 s1' H1 s2 s2' H2.
+    unfold_eq_universe. specialize (H1 v Hv). specialize (H2 v Hv).
+    rewrite !val_sup; lia.
+  Qed.
+
+  Lemma sort_of_product_twice φ u s :
+    eq_universe φ (Universe.sort_of_product u (Universe.sort_of_product u s))
+                (Universe.sort_of_product u s).
+  Proof.
+    unfold Universe.sort_of_product. case_eq (Universe.is_prop s).
+    intros ->. reflexivity.
+    intro e. rewrite is_prop_sup e andb_false_r.
+    rewrite eq_universe_sup_assoc.
+    rewrite eq_universe_sup_idem.
+    reflexivity.
+  Qed.
+
+End UniverseLemmas.
